SeparationLogic/Semantics.v
@@ -13,7 +13,7 @@ Local Open Scope SeparationLogic.
 
 Module DownwardsSemantics.
 
-Class DownwardsSemantics (L: Language) {nL: NormalLanguage L} {pL: PropositionalLanguage L} {SL: SeparationLanguage L} (MD: Model) {kMD: KripkeModel MD} (M: Kmodel) {kiM: KripkeIntuitionisticModel MD M} {SA: SeparationAlgebra MD M} (SM: Semantics L MD) {kiSM: KripkeIntuitionisticSemantics L MD M SM}: Type := {
+Class DownwardsSemantics (L: Language) {nL: NormalLanguage L} {pL: PropositionalLanguage L} {SL: SeparationLanguage L} (MD: Model) {kMD: KripkeModel MD} (M: Kmodel) {kiM: KripkeIntuitionisticModel (Kworlds M)} {SA: SeparationAlgebra (Kworlds M)} (SM: Semantics L MD) {kiSM: KripkeIntuitionisticSemantics L MD M SM}: Type := {
   sat_sepcon: forall m x y, KRIPKE: M , m |= x * y <-> exists m1 m2, join m1 m2 m /\ KRIPKE: M , m1 |= x /\ KRIPKE: M, m2 |= y;
   sat_wand: forall m x y, KRIPKE: M , m |= x -* y <-> forall m0 m1 m2, m0 <= m -> join m0 m1 m2 -> KRIPKE: M , m1 |= x -> KRIPKE: M, m2 |= y
 }.
@@ -22,7 +22,7 @@ End DownwardsSemantics.
 
 Module UpwardsSemantics.
 
-Class UpwardsSemantics (L: Language) {nL: NormalLanguage L} {pL: PropositionalLanguage L} {SL: SeparationLanguage L} (MD: Model) {kMD: KripkeModel MD} (M: Kmodel) {kiM: KripkeIntuitionisticModel MD M} {SA: SeparationAlgebra MD M} (SM: Semantics L MD) {kiSM: KripkeIntuitionisticSemantics L MD M SM}: Type := {
+Class UpwardsSemantics (L: Language) {nL: NormalLanguage L} {pL: PropositionalLanguage L} {SL: SeparationLanguage L} (MD: Model) {kMD: KripkeModel MD} (M: Kmodel) {kiM: KripkeIntuitionisticModel (Kworlds M)} {SA: SeparationAlgebra (Kworlds M)} (SM: Semantics L MD) {kiSM: KripkeIntuitionisticSemantics L MD M SM}: Type := {
   sat_sepcon: forall m x y, KRIPKE: M , m |= x * y <-> exists m0 m1 m2, m <= m0 /\ join m1 m2 m0 /\ KRIPKE: M , m1 |= x /\ KRIPKE: M, m2 |= y;
   sat_wand: forall m x y, KRIPKE: M , m |= x -* y <-> forall m1 m2, join m m1 m2 -> KRIPKE: M , m1 |= x -> KRIPKE: M, m2 |= y
 }.
@@ -31,14 +31,14 @@ End UpwardsSemantics.
 
 Module FlatSemantics.
 
-Class FlatSemantics (L: Language) {nL: NormalLanguage L} {pL: PropositionalLanguage L} {SL: SeparationLanguage L} (MD: Model) {kMD: KripkeModel MD} (M: Kmodel) {kiM: KripkeIntuitionisticModel MD M} {SA: SeparationAlgebra MD M} (SM: Semantics L MD) {kiSM: KripkeIntuitionisticSemantics L MD M SM}: Type := {
+Class FlatSemantics (L: Language) {nL: NormalLanguage L} {pL: PropositionalLanguage L} {SL: SeparationLanguage L} (MD: Model) {kMD: KripkeModel MD} (M: Kmodel) {kiM: KripkeIntuitionisticModel (Kworlds M)} {SA: SeparationAlgebra (Kworlds M)} (SM: Semantics L MD) {kiSM: KripkeIntuitionisticSemantics L MD M SM}: Type := {
   sat_sepcon: forall m x y, KRIPKE: M , m |= x * y <-> exists m1 m2, join m1 m2 m /\ KRIPKE: M , m1 |= x /\ KRIPKE: M, m2 |= y;
   sat_wand: forall m x y, KRIPKE: M , m |= x -* y <-> forall m1 m2, join m m1 m2 -> KRIPKE: M , m1 |= x -> KRIPKE: M, m2 |= y
 }.
 
 End FlatSemantics.
 
-Class UnitarySemantics (L: Language) {nL: NormalLanguage L} {pL: PropositionalLanguage L} {SL: SeparationLanguage L} {uSL: UnitarySeparationLanguage L} (MD: Model) {kMD: KripkeModel MD} (M: Kmodel) {kiM: KripkeIntuitionisticModel MD M} {SA: SeparationAlgebra MD M} {USA: UnitarySeparationAlgebra MD M} (SM: Semantics L MD) {kiSM: KripkeIntuitionisticSemantics L MD M SM}: Type := {
+Class UnitarySemantics (L: Language) {nL: NormalLanguage L} {pL: PropositionalLanguage L} {SL: SeparationLanguage L} {uSL: UnitarySeparationLanguage L} (MD: Model) {kMD: KripkeModel MD} (M: Kmodel) {kiM: KripkeIntuitionisticModel (Kworlds M)} {SA: SeparationAlgebra (Kworlds M)} {USA: UnitarySeparationAlgebra (Kworlds M)} (SM: Semantics L MD) {kiSM: KripkeIntuitionisticSemantics L MD M SM}: Type := {
   sat_emp: forall (m: Kworlds M), KRIPKE: M, m |= emp <-> unit m
 }.
 
