SeparationLogic/SeparationAlgebra.v
@@ -5,32 +5,35 @@ Require Import Logic.PropositionalLogic.KripkeSemantics.
 
 Local Open Scope KripkeSemantics.
 
-Class SeparationAlgebra (MD: Model) {kMD: KripkeModel MD} (M: Kmodel): Type := {
-  join: Kworlds M -> Kworlds M -> Kworlds M -> Prop;
-  join_comm: forall m1 m2 m: Kworlds M, join m1 m2 m -> join m2 m1 m;
-  join_assoc: forall mx my mz mxy mxyz: Kworlds M, join mx my mxy -> join mxy mz mxyz -> exists myz, join my mz myz /\ join mx myz mxyz
+Class SeparationAlgebra (worlds: Type): Type := {
+  join: worlds -> worlds -> worlds -> Prop
 }.
 
-Class GarbageCollectSeparationAlgebra (MD: Model) {kMD: KripkeModel MD} (M: Kmodel) {kiM: KripkeIntuitionisticModel MD M} {SA: SeparationAlgebra MD M}: Type := {
-  join_has_order1: forall (m1 m2 m: Kworlds M), join m1 m2 m -> m <= m1
+Class NormalSeparationAlgebra (worlds: Type) {SA: SeparationAlgebra worlds}: Type := {
+  join_comm: forall m1 m2 m: worlds, join m1 m2 m -> join m2 m1 m;
+  join_assoc: forall mx my mz mxy mxyz: worlds, join mx my mxy -> join mxy mz mxyz -> exists myz, join my mz myz /\ join mx myz mxyz
 }.
 
-Class UnitarySeparationAlgebra (MD: Model) {kMD: KripkeModel MD} (M: Kmodel) {kiM: KripkeIntuitionisticModel MD M} {SA: SeparationAlgebra MD M}: Type := {
-  unit: Kworlds M -> Prop;
-  unit_spec: forall m: Kworlds M, unit m <-> forall n n', join m n n' -> n' <= n;
-  unit_exists: forall n: Kworlds M, exists m, join m n n /\ unit m
+Class GarbageCollectSeparationAlgebra (worlds: Type) {kiM: KripkeIntuitionisticModel worlds} {SA: SeparationAlgebra worlds}: Type := {
+  join_has_order1: forall (m1 m2 m: worlds), join m1 m2 m -> m <= m1
 }.
 
-Class NormalUnitarySeparationAlgebra (MD: Model) {kMD: KripkeModel MD} (M: Kmodel) {kiM: KripkeIntuitionisticModel MD M} {SA: SeparationAlgebra MD M} {USA: UnitarySeparationAlgebra MD M}: Type := {
-  unit_down: forall n m: Kworlds M, n <= m -> unit m -> unit n
+Class UnitarySeparationAlgebra (worlds: Type) {kiM: KripkeIntuitionisticModel worlds} {SA: SeparationAlgebra worlds}: Type := {
+  unit: worlds -> Prop;
+  unit_spec: forall m: worlds, unit m <-> forall n n', join m n n' -> n' <= n;
+  unit_exists: forall n: worlds, exists m, join m n n /\ unit m
 }.
 
-Class DownwardsClosedSeparationAlgebra (MD: Model) {kMD: KripkeModel MD} (M: Kmodel) {kiM: KripkeIntuitionisticModel MD M} {SA: SeparationAlgebra MD M}: Type := {
-  join_Korder_down: forall (m n m1 m2: Kworlds M), join m1 m2 m -> n <= m -> exists n1 n2, join n1 n2 n /\ n1 <= m1 /\ n2 <= m2
+Class NormalUnitarySeparationAlgebra (worlds: Type) {kiM: KripkeIntuitionisticModel worlds} {SA: SeparationAlgebra worlds} {USA: UnitarySeparationAlgebra worlds}: Type := {
+  unit_down: forall n m: worlds, n <= m -> unit m -> unit n
 }.
 
-Class UpwardsClosedSeparationAlgebra (MD: Model) {kMD: KripkeModel MD} (M: Kmodel) {kiM: KripkeIntuitionisticModel MD M} {SA: SeparationAlgebra MD M}: Type := {
-  join_Korder_up: forall (m1 m2 m n1 n2: Kworlds M), join m1 m2 m -> m1 <= n1 -> m2 <= n2 -> exists n, join n1 n2 n /\ m <= n
+Class DownwardsClosedSeparationAlgebra (worlds: Type) {kiM: KripkeIntuitionisticModel worlds} {SA: SeparationAlgebra worlds}: Type := {
+  join_Korder_down: forall m n m1 m2: worlds, join m1 m2 m -> n <= m -> exists n1 n2, join n1 n2 n /\ n1 <= m1 /\ n2 <= m2
+}.
+
+Class UpwardsClosedSeparationAlgebra (worlds: Type) {kiM: KripkeIntuitionisticModel worlds} {SA: SeparationAlgebra worlds}: Type := {
+  join_Korder_up: forall m1 m2 m n1 n2: worlds, join m1 m2 m -> m1 <= n1 -> m2 <= n2 -> exists n, join n1 n2 n /\ m <= n
 }.
 
 (* David J. Pym, Peter W. O’Hearn, and Hongseok Yang. Possible worlds and resources: the semantics of BI. *)
@@ -41,7 +44,7 @@ Class UpwardsClosedSeparationAlgebra (MD: Model) {kMD: KripkeModel MD} (M: Kmode
 It is necessary to be this strong, or else sepcon_assoc will be unsound, e.g. the following weaker version causes unsoundness:
   join_Korder: forall M (m1 m2 m n1: Kworlds M), join m1 m2 m -> Korder m1 n1 -> exists n2 n, join n1 n2 n /\ Korder m2 n2 /\ Korder m n;  *)
 
-Definition UpwardsClosed_nUSA {MD: Model} {kMD: KripkeModel MD} (M: Kmodel) {kiM: KripkeIntuitionisticModel MD M} {SA: SeparationAlgebra MD M} {uSA: UpwardsClosedSeparationAlgebra MD M} {USA: UnitarySeparationAlgebra MD M}: NormalUnitarySeparationAlgebra MD M.
+Definition UpwardsClosed_nUSA (worlds: Type) {kiM: KripkeIntuitionisticModel worlds} {SA: SeparationAlgebra worlds} {uSA: UpwardsClosedSeparationAlgebra worlds} {USA: UnitarySeparationAlgebra worlds}: NormalUnitarySeparationAlgebra worlds.
 Proof.
   constructor.
   intros.
