SeparationLogic/SeparationAlgebraConstruction.v
@@ -7,9 +7,12 @@ Require Import Logic.SeparationLogic.SeparationAlgebra.
 Local Open Scope logic_base.
 Local Open Scope KripkeSemantics.
 
-Definition DownwardsClosure_SA {MD: Model} {kMD: KripkeModel MD} (M: Kmodel) {kiM: KripkeIntuitionisticModel MD M} {SA: SeparationAlgebra MD M} {uSA: UpwardsClosedSeparationAlgebra MD M}: SeparationAlgebra MD M.
+Definition DownwardsClosure_SA (worlds: Type) {kiM: KripkeIntuitionisticModel worlds} {SA: SeparationAlgebra worlds}: SeparationAlgebra worlds :=
+  Build_SeparationAlgebra _ (fun m1 m2 m: worlds => exists n, Korder m n /\ join m1 m2 n).
+
+Definition DownwardsClosure_nSA {worlds: Type} {kiM: KripkeIntuitionisticModel worlds} {SA: SeparationAlgebra worlds} {nSA: NormalSeparationAlgebra worlds} {uSA: UpwardsClosedSeparationAlgebra worlds}: @NormalSeparationAlgebra worlds (DownwardsClosure_SA worlds).
 Proof.
-  apply (Build_SeparationAlgebra _ _ _ (fun (m1 m2 m: Kworlds M) => exists n, Korder m n /\ join m1 m2 n)).
+  constructor.
   + intros.
     destruct H as [n [? ?]].
     exists n.
@@ -30,9 +33,9 @@ Proof.
       etransitivity; eauto.
 Defined.
 
-Definition DownwardsClosure_USA {MD: Model} {kMD: KripkeModel MD} (M: Kmodel) {kiM: KripkeIntuitionisticModel MD M} {SA: SeparationAlgebra MD M} {uSA: UpwardsClosedSeparationAlgebra MD M} {USA: UnitarySeparationAlgebra MD M} {nUSA: NormalUnitarySeparationAlgebra MD M}: @UnitarySeparationAlgebra MD _ M _ (DownwardsClosure_SA M).
+Definition DownwardsClosure_USA (worlds: Type) {kiM: KripkeIntuitionisticModel worlds} {SA: SeparationAlgebra worlds} {nSA: NormalSeparationAlgebra worlds} {uSA: UpwardsClosedSeparationAlgebra worlds} {USA: UnitarySeparationAlgebra worlds} {nUSA: NormalUnitarySeparationAlgebra worlds}: @UnitarySeparationAlgebra worlds _ (DownwardsClosure_SA worlds).
 Proof.
-  apply (Build_UnitarySeparationAlgebra _ _ _ _ _ unit).
+  apply (Build_UnitarySeparationAlgebra _ _ _ unit).
   + intros.
     simpl.
     pose proof Korder_PreOrder as H_PreOrder.
@@ -53,7 +56,7 @@ Proof.
     reflexivity.
 Defined.
 
-Definition DownwardsClosure_DownwardsClosed {MD: Model} {kMD: KripkeModel MD} (M: Kmodel) {kiM: KripkeIntuitionisticModel MD M} {SA: SeparationAlgebra MD M} {uSA: UpwardsClosedSeparationAlgebra MD M}: @DownwardsClosedSeparationAlgebra MD _ M _ (DownwardsClosure_SA M).
+Definition DownwardsClosure_DownwardsClosed {worlds: Type} {kiM: KripkeIntuitionisticModel worlds} {SA: SeparationAlgebra worlds} {nSA: NormalSeparationAlgebra worlds} {uSA: UpwardsClosedSeparationAlgebra worlds}: @DownwardsClosedSeparationAlgebra worlds _ (DownwardsClosure_SA worlds).
 Proof.
   constructor.
   intros.
@@ -65,7 +68,7 @@ Proof.
   split; auto; etransitivity; eauto.
 Defined.
 
-Definition DownwardsClosure_UpwardsClosed {MD: Model} {kMD: KripkeModel MD} (M: Kmodel) {kiM: KripkeIntuitionisticModel MD M} {SA: SeparationAlgebra MD M} {uSA: UpwardsClosedSeparationAlgebra MD M}: @UpwardsClosedSeparationAlgebra MD _ M _ (DownwardsClosure_SA M).
+Definition DownwardsClosure_UpwardsClosed {worlds: Type} {kiM: KripkeIntuitionisticModel worlds} {SA: SeparationAlgebra worlds} {nSA: NormalSeparationAlgebra worlds} {uSA: UpwardsClosedSeparationAlgebra worlds}: @UpwardsClosedSeparationAlgebra worlds _ (DownwardsClosure_SA worlds).
 Proof.
   constructor.
   intros.
@@ -77,14 +80,14 @@ Proof.
   exists n'; split; auto.
 Defined.
 
-Definition DownwardsClosure_nUSA {MD: Model} {kMD: KripkeModel MD} (M: Kmodel) {kiM: KripkeIntuitionisticModel MD M} {SA: SeparationAlgebra MD M} {uSA: UpwardsClosedSeparationAlgebra MD M} {USA: UnitarySeparationAlgebra MD M} {nUSA: NormalUnitarySeparationAlgebra MD M}: @NormalUnitarySeparationAlgebra MD _ M _ (DownwardsClosure_SA M) (DownwardsClosure_USA M).
+Definition DownwardsClosure_nUSA {worlds: Type} {kiM: KripkeIntuitionisticModel worlds} {SA: SeparationAlgebra worlds} {nSA: NormalSeparationAlgebra worlds} {uSA: UpwardsClosedSeparationAlgebra worlds} {USA: UnitarySeparationAlgebra worlds} {nUSA: NormalUnitarySeparationAlgebra worlds}: @NormalUnitarySeparationAlgebra worlds _ (DownwardsClosure_SA worlds) (DownwardsClosure_USA worlds).
 Proof.
   constructor.
   simpl.
   apply unit_down.
 Qed.
 
-Definition DownwardsClosure_gcSA {MD: Model} {kMD: KripkeModel MD} (M: Kmodel) {kiM: KripkeIntuitionisticModel MD M} {SA: SeparationAlgebra MD M} {uSA: UpwardsClosedSeparationAlgebra MD M} {USA: UnitarySeparationAlgebra MD M} {nUSA: NormalUnitarySeparationAlgebra MD M} {gcSA: GarbageCollectSeparationAlgebra MD M}: @GarbageCollectSeparationAlgebra MD _ M _ (DownwardsClosure_SA M).
+Definition DownwardsClosure_gcSA {worlds: Type} {kiM: KripkeIntuitionisticModel worlds} {SA: SeparationAlgebra worlds} {nSA: NormalSeparationAlgebra worlds} {uSA: UpwardsClosedSeparationAlgebra worlds} {gcSA: GarbageCollectSeparationAlgebra worlds}: @GarbageCollectSeparationAlgebra worlds _ (DownwardsClosure_SA worlds).
 Proof.
   constructor.
   simpl.
@@ -95,9 +98,12 @@ Proof.
   eapply join_has_order1; eauto.
 Qed.
 
-Definition UpwardsClosure_SA {MD: Model} {kMD: KripkeModel MD} (M: Kmodel) {kiM: KripkeIntuitionisticModel MD M} {SA: SeparationAlgebra MD M} {dSA: DownwardsClosedSeparationAlgebra MD M}: SeparationAlgebra MD M.
+Definition UpwardsClosure_SA (worlds: Type) {kiM: KripkeIntuitionisticModel worlds} {SA: SeparationAlgebra worlds}: SeparationAlgebra worlds :=
+  Build_SeparationAlgebra _ (fun m1 m2 m: worlds => exists n1 n2, n1 <= m1 /\ n2 <= m2 /\ join n1 n2 m).
+
+Definition UpwardsClosure_nSA {worlds: Type} {kiM: KripkeIntuitionisticModel worlds} {SA: SeparationAlgebra worlds} {nSA: NormalSeparationAlgebra worlds} {dSA: DownwardsClosedSeparationAlgebra worlds}: @NormalSeparationAlgebra worlds (UpwardsClosure_SA worlds).
 Proof.
-  apply (Build_SeparationAlgebra _ _ _ (fun (m1 m2 m: Kworlds M) => exists n1 n2, n1 <= m1 /\ n2 <= m2 /\ join n1 n2 m)).
+  constructor.
   + (* join_comm *)
     intros.
     destruct H as [n1 [n2 [? [? ?]]]].
@@ -120,9 +126,9 @@ Proof.
       * reflexivity.
 Defined.
 
-Definition UpwardsClosure_USA {MD: Model} {kMD: KripkeModel MD} (M: Kmodel) {kiM: KripkeIntuitionisticModel MD M} {SA: SeparationAlgebra MD M} {dSA: DownwardsClosedSeparationAlgebra MD M} {USA: UnitarySeparationAlgebra MD M} {nUSA: NormalUnitarySeparationAlgebra MD M}: @UnitarySeparationAlgebra MD _ M _ (UpwardsClosure_SA M).
+Definition UpwardsClosure_USA (worlds: Type) {kiM: KripkeIntuitionisticModel worlds} {SA: SeparationAlgebra worlds} {nSA: NormalSeparationAlgebra worlds} {dSA: DownwardsClosedSeparationAlgebra worlds} {USA: UnitarySeparationAlgebra worlds} {nUSA: NormalUnitarySeparationAlgebra worlds}: @UnitarySeparationAlgebra worlds _ (UpwardsClosure_SA worlds).
 Proof.
-  apply (Build_UnitarySeparationAlgebra _ _ _ _ _ unit).
+  apply (Build_UnitarySeparationAlgebra _ _ _ unit).
   + intros.
     simpl.
     pose proof Korder_PreOrder as H_PreOrder.
@@ -143,7 +149,7 @@ Proof.
     exists u, n; split; [| split]; auto; reflexivity.
 Defined.
 
-Definition UpwardsClosure_UpwardsClosed {MD: Model} {kMD: KripkeModel MD} (M: Kmodel) {kiM: KripkeIntuitionisticModel MD M} {SA_D: SeparationAlgebra MD M} {dSA: DownwardsClosedSeparationAlgebra MD M}: @UpwardsClosedSeparationAlgebra MD _ M _ (UpwardsClosure_SA M).
+Definition UpwardsClosure_UpwardsClosed {worlds: Type} {kiM: KripkeIntuitionisticModel worlds} {SA: SeparationAlgebra worlds} {nSA: NormalSeparationAlgebra worlds} {dSA: DownwardsClosedSeparationAlgebra worlds}: @UpwardsClosedSeparationAlgebra worlds _ (UpwardsClosure_SA worlds).
 Proof.
   constructor.
   intros.
@@ -155,7 +161,7 @@ Proof.
   split; [| split]; auto; etransitivity; eauto.
 Qed.
 
-Definition UpwardsClosure_DownwardsClosed {MD: Model} {kMD: KripkeModel MD} (M: Kmodel) {kiM: KripkeIntuitionisticModel MD M} {SA_D: SeparationAlgebra MD M} {dSA: DownwardsClosedSeparationAlgebra MD M}: @DownwardsClosedSeparationAlgebra MD _ M _ (UpwardsClosure_SA M).
+Definition UpwardsClosure_DownwardsClosed {worlds: Type} {kiM: KripkeIntuitionisticModel worlds} {SA: SeparationAlgebra worlds} {nSA: NormalSeparationAlgebra worlds} {dSA: DownwardsClosedSeparationAlgebra worlds}: @DownwardsClosedSeparationAlgebra worlds _ (UpwardsClosure_SA worlds).
 Proof.
   constructor.
   intros.
@@ -167,14 +173,14 @@ Proof.
   exists n1', n2'; split; [| split]; auto.
 Qed.
 
-Definition UpwardsClosure_nUSA {MD: Model} {kMD: KripkeModel MD} (M: Kmodel) {kiM: KripkeIntuitionisticModel MD M} {SA: SeparationAlgebra MD M} {dSA: DownwardsClosedSeparationAlgebra MD M} {USA: UnitarySeparationAlgebra MD M} {nUSA: NormalUnitarySeparationAlgebra MD M}: @NormalUnitarySeparationAlgebra MD _ M _ (UpwardsClosure_SA M) (UpwardsClosure_USA M).
+Definition UpwardsClosure_nUSA {worlds: Type} {kiM: KripkeIntuitionisticModel worlds} {SA: SeparationAlgebra worlds} {nSA: NormalSeparationAlgebra worlds} {dSA: DownwardsClosedSeparationAlgebra worlds} {USA: UnitarySeparationAlgebra worlds} {nUSA: NormalUnitarySeparationAlgebra worlds}: @NormalUnitarySeparationAlgebra worlds _ (UpwardsClosure_SA worlds) (UpwardsClosure_USA worlds).
 Proof.
   constructor.
   simpl.
   apply unit_down.
 Qed.
 
-Definition UpwardsClosure_gcSA {MD: Model} {kMD: KripkeModel MD} (M: Kmodel) {kiM: KripkeIntuitionisticModel MD M} {SA: SeparationAlgebra MD M} {dSA: DownwardsClosedSeparationAlgebra MD M} {USA: UnitarySeparationAlgebra MD M} {nUSA: NormalUnitarySeparationAlgebra MD M} {gcSA: GarbageCollectSeparationAlgebra MD M}: @GarbageCollectSeparationAlgebra MD _ M _ (UpwardsClosure_SA M).
+Definition UpwardsClosure_gcSA {worlds: Type} {kiM: KripkeIntuitionisticModel worlds} {SA: SeparationAlgebra worlds} {nSA: NormalSeparationAlgebra worlds} {dSA: DownwardsClosedSeparationAlgebra worlds} {gcSA: GarbageCollectSeparationAlgebra worlds}: @GarbageCollectSeparationAlgebra worlds _ (UpwardsClosure_SA worlds).
 Proof.
   constructor.
   simpl.
