SeparationLogic/Sound_DownUp_Fail.v
@@ -14,7 +14,7 @@ Local Open Scope PropositionalLogic.
 Local Open Scope SeparationLogic.
 Local Open Scope KripkeSemantics.
 
-Lemma sound_sepcon_comm {L: Language} {nL: NormalLanguage L} {pL: PropositionalLanguage L} {SL: SeparationLanguage L} {MD: Model} {kMD: KripkeModel MD} (M: Kmodel) {kiM: KripkeIntuitionisticModel MD M} {SA: SeparationAlgebra MD M} {SM: Semantics L MD} {kiSM: KripkeIntuitionisticSemantics L MD M SM} {dusSM: DownUpSemantics L MD M SM}:
+Lemma sound_sepcon_comm {L: Language} {nL: NormalLanguage L} {pL: PropositionalLanguage L} {SL: SeparationLanguage L} {MD: Model} {kMD: KripkeModel MD} (M: Kmodel) {kiM: KripkeIntuitionisticModel (Kworlds M)} {SA: SeparationAlgebra (Kworlds M)} {nSA: NormalSeparationAlgebra (Kworlds M)} {SM: Semantics L MD} {kiSM: KripkeIntuitionisticSemantics L MD M SM} {dusSM: DownUpSemantics L MD M SM}:
   forall x y: expr,
     forall m,
       KRIPKE: M, m |= x * y --> y * x.
@@ -29,7 +29,7 @@ Proof.
   apply join_comm; auto.
 Qed.
 
-Lemma sound_sepcon_assoc {L: Language} {nL: NormalLanguage L} {pL: PropositionalLanguage L} {SL: SeparationLanguage L} {MD: Model} {kMD: KripkeModel MD} (M: Kmodel) {kiM: KripkeIntuitionisticModel MD M} {SA: SeparationAlgebra MD M} {SM: Semantics L MD} {kiSM: KripkeIntuitionisticSemantics L MD M SM} {dusSM: DownUpSemantics L MD M SM}:
+Lemma sound_sepcon_assoc {L: Language} {nL: NormalLanguage L} {pL: PropositionalLanguage L} {SL: SeparationLanguage L} {MD: Model} {kMD: KripkeModel MD} (M: Kmodel) {kiM: KripkeIntuitionisticModel (Kworlds M)} {SA: SeparationAlgebra (Kworlds M)} {nSA: NormalSeparationAlgebra (Kworlds M)} {SM: Semantics L MD} {kiSM: KripkeIntuitionisticSemantics L MD M SM} {dusSM: DownUpSemantics L MD M SM}:
   forall x y z: expr,
     forall m,
       KRIPKE: M, m |= x * (y * z) <--> (x * y) * z.
